Setlec.lean
@@ -22,6 +22,7 @@ import Setlec.Model.ProjInstall
 import Setlec.Model.DirectTower
 import Setlec.Model.DirectInstall
 import Setlec.Model.DirectParams
+import Setlec.Model.DirectExtend
 import Setlec.Model.Extend
 import Setlec.Model.Consistency
 import Setlec.Verify.Mono
